@prefix rdfs:  <http://www.w3.org/2000/01/rdf-schema#> .
@prefix owl:   <http://www.w3.org/2002/07/owl#> .
@prefix xsd:   <http://www.w3.org/2001/XMLSchema#> .
@prefix rdf:   <http://www.w3.org/1999/02/22-rdf-syntax-ns#> .
@prefix qb:    <http://purl.org/linked-data/cube#> .
@prefix skos:  <http://www.w3.org/2004/02/skos/core#> .
@prefix dcterms: <http://purl.org/dc/terms/> .

<http://data.gmdsp.org.uk/def/council/allotment/Plot>
        rdfs:label       "Part of an allotment which has been split into smaller areas"^^xsd:string ;
        rdfs:subClassOf  <http://data.smartcityconceptmodel.com/model#Object> ;
        rdfs:isDefinedBy <http://data.gmdsp.org.uk/def/council/allotment> .

<http://data.gmdsp.org.uk/def/council/allotment/rent>
        a             <http://purl.org/goodrelations/v1#UnitPriceSpecification> ;
        rdfs:comment  "How much does it cost to rent the allotment" ;
        rdfs:domain   <http://data.gmdsp.org.uk/def/council/Allotment> ;
        rdfs:label    "Rent"^^xsd:string ;
        rdfs:isDefinedBy <http://data.gmdsp.org.uk/def/council/allotment> .

<http://data.gmdsp.org.uk/def/council/allotment/number-of-plots>
        a             rdfs:Property ;
        rdfs:comment  "Number of plots which the allotment has"^^xsd:string ;
        rdfs:domain   <http://data.gmdsp.org.uk/def/council/Allotment> ;
        rdfs:label    "Number of plots"^^xsd:string ;
        rdfs:range    xsd:integer ;
        rdfs:isDefinedBy <http://data.gmdsp.org.uk/def/council/allotment> .

<http://data.gmdsp.org.uk/def/council/allotment/information-page>
        a                   rdfs:Property ;
        rdfs:comment        "Page (given by URL) where further information for this allotment."^^xsd:string ;
        rdfs:domain         <http://data.gmdsp.org.uk/def/council/Allotment> ;
        rdfs:label          "Information page"^^xsd:string ;
        rdfs:subPropertyOf  <http://xmlns.com/foaf/0.1/page> ;
        rdfs:isDefinedBy <http://data.gmdsp.org.uk/def/council/allotment> .

<http://data.gmdsp.org.uk/def/council/allotment/disabled-access>
        a             rdfs:Property ;
        rdfs:comment  "Does the allotment have disabled access"^^xsd:string ;
        rdfs:domain   <http://data.gmdsp.org.uk/def/council/Allotment> ;
        rdfs:label    "Disabled access"^^xsd:string ;
        rdfs:range    xsd:boolean ;
        rdfs:isDefinedBy <http://data.gmdsp.org.uk/def/council/allotment> .

<http://data.gmdsp.org.uk/def/council/allotment/plot-size>
        a             rdfs:Property ;
        rdfs:comment  "How big is the allotment plot in square meters"^^xsd:string ;
        rdfs:domain   <http://data.gmdsp.org.uk/def/council/Allotment> ;
        rdfs:label    "Plot size"^^xsd:string ;
        rdfs:range    <http://qudt.org/vocab/unit/squareMeter> ;
        rdfs:isDefinedBy <http://data.gmdsp.org.uk/def/council/allotment> .

<http://data.gmdsp.org.uk/def/council/allotment/hasPlot>
        rdfs:comment  "Each allotment can have a number of plots, each of which can be uniquely defined"^^xsd:string ;
        rdfs:domain   <http://data.gmdsp.org.uk/def/council/Allotment> ;
        rdfs:label    "A plot belongs to an allotment"^^xsd:string ;
        rdfs:range    <http://data.gmdsp.org.uk/def/council/Plot> ;
        <http://www.w3.org/2000/01/rdf-schema#type:>
                rdfs:Property ;
                rdfs:isDefinedBy <http://data.gmdsp.org.uk/def/council/allotment> .

<http://data.gmdsp.org.uk/def/council/allotment/application-page>
        a                   rdfs:Property ;
        rdfs:comment        "Page (given by URL) with application information for this allotment."^^xsd:string ;
        rdfs:domain         <http://data.gmdsp.org.uk/def/council/Allotment> ;
        rdfs:label          "Application page"^^xsd:string ;
        rdfs:subPropertyOf  <http://xmlns.com/foaf/0.1/page> ;
        rdfs:isDefinedBy <http://data.gmdsp.org.uk/def/council/allotment> .

<http://data.gmdsp.org.uk/def/council/allotment/guidance-page>
        a                   rdfs:Property ;
        rdfs:comment        "Page (given by URL) with guidance for this allotment."^^xsd:string ;
        rdfs:domain         <http://data.gmdsp.org.uk/def/council/Allotment> ;
        rdfs:label          "Guidance page"^^xsd:string ;
        rdfs:subPropertyOf  <http://xmlns.com/foaf/0.1/page> ;
        rdfs:isDefinedBy <http://data.gmdsp.org.uk/def/council/allotment> .

<http://data.gmdsp.org.uk/def/council/allotment/Allotment>
        a                rdfs:Class, owl:Class ;
        rdfs:label       "An RDF class to describe an Allotment"^^xsd:string ;
        rdfs:subClassOf  <http://data.smartcityconceptmodel.com/model#Object> ;
        rdfs:isDefinedBy <http://data.gmdsp.org.uk/def/council/allotment> .

<http://gmdsp.org/def/statistical-dimension/allotments/refAllotment> 
        a                rdfs:Property ;
        rdfs:label       "The allotment instance being referred to."^^xsd:string ;
        rdfs:comment     "Used when referring to an allotment measure in an observation" ;
        rdfs:isDefinedBy <http://gmdsp.org/def/statistical-dimension/allotments>  .

<http://gmdsp.org/def/statistical-dimension/allotments/inUse> 
        a                rdfs:Property ;
        rdfs:label       "The allotment usage"^^xsd:string ;
        rdfs:comment     "Used when referring to allotment usage at one particular moment in time in an statistical observation" ;
        rdfs:isDefinedBy <http://gmdsp.org/def/statistical-dimension/allotments>  .

<http://gmdsp.org/def/statistical-dimension/allotments/untenable> 
        a                rdfs:Property ;
        rdfs:label       "The amount of allotment plots which are untenable"^^xsd:string ;
        rdfs:comment     "Used when referring to the amount of allotment plots which are untenable at one particular moment in time in an statistical observation" ;
        rdfs:isDefinedBy <http://gmdsp.org/def/statistical-dimension/allotments>  .

<http://gmdsp.org/def/statistical-dimension/allotments/vacant> 
        a                rdfs:Property ;
        rdfs:label       "The amount of allotment plots which are vacant"^^xsd:string ;
        rdfs:comment     "Used when referring to the amount of allotment plots which are vacant at one particular moment in time in an statistical observation" ;
        rdfs:isDefinedBy <http://gmdsp.org/def/statistical-dimension/allotments>  .

<http://gmdsp.org/def/statistical-dimension/allotments/notice> 
        a                rdfs:Property ;
        rdfs:label       "The amount of allotment plots who's renters have been given notice"^^xsd:string ;
        rdfs:comment     "Used when referring to the amount of allotment plots who's current renters have been served notice to vacate at one particular moment in time in an statistical observation" ;
        rdfs:isDefinedBy <http://gmdsp.org/def/statistical-dimension/allotments>  .

<http://gmdsp.org/def/statistical-dimension/allotments/waiting> 
        a                rdfs:Property ;
        rdfs:label       "The number of people on the waiting list for an alotment"^^xsd:string ;
        rdfs:comment     "Used when referring to the number of people on the waiting list at an allotment at one particular moment in time in an statistical observation" ;
        rdfs:isDefinedBy <http://gmdsp.org/def/statistical-dimension/allotments>  .