@prefix rdf: <http://www.w3.org/1999/02/22-rdf-syntax-ns#> .
@prefix xsd: <http://www.w3.org/2001/XMLSchema#> .
@prefix rdfs: <http://www.w3.org/2000/01/rdf-schema#> .
@prefix smartcity: <http://data.smartcityconceptmodel.com/model#> .

#################################################################
#
#    Classes
#
#################################################################

<http://data.gmdsp.org.uk/def/council/planning/PlanningApplication>
      rdfs:label "Planning application"^^xsd:string ;
      rdfs:subClassOf smartcity:Object ;
      rdfs:isDefinedBy <http://data.gmdsp.org.uk/def/council/planning> .

<http://data.gmdsp.org.uk/def/council/planning/PlanningApplicationSite>
      rdfs:label "Planning application site"^^xsd:string ;
      rdfs:subClassOf smartcity:Object ;
      rdfs:isDefinedBy <http://data.gmdsp.org.uk/def/council/planning> .


#################################################################
#
#    Properties
#
#################################################################

<http://data.gmdsp.org.uk/def/council/planning/decision>
      rdf:type rdf:Property ;
      rdfs:label "Planning decision"^^xsd:string ;
	  rdfs:comment "What the outcome of a planning applications was. Will have one decision as defined in a concept scheme." ;
      rdfs:domain <http://data.gmdsp.org.uk/def/council/planning/PlanningApplication> ;
      rdfs:range <http://data.gmdsp.org.uk/def/council/planning/planning-application-status> .

<http://data.gmdsp.org.uk/def/council/planning/validatedDate>
      rdf:type rdf:Property ;
      rdfs:label "Validated date"^^xsd:string ;
	  rdfs:comment "Date the planning application was validated and accepted." ;
      rdfs:domain <http://data.gmdsp.org.uk/def/council/planning/PlanningApplication> ;
      rdfs:range xsd:date .

<http://data.gmdsp.org.uk/def/council/planning/decisionDate>
      rdf:type rdf:Property ;
      rdfs:label "Decision date"^^xsd:string ;
	  rdfs:comment "Date the planning application decision was made." ;
      rdfs:domain <http://data.gmdsp.org.uk/def/council/planning/PlanningApplication> ;
      rdfs:range xsd:date .

<http://data.gmdsp.org.uk/def/council/planning/applicationType>
      rdf:type rdf:Property ;
      rdfs:label "Application type"^^xsd:string ;
	  rdfs:comment "Long form version of the application type eg advertisement (see also developmentType)." ;
      rdfs:domain <http://data.gmdsp.org.uk/def/council/planning/PlanningApplication> ;
      rdfs:range <http://data.gmdsp.org.uk/def/council/planning/planning-application-type> .

<http://data.gmdsp.org.uk/def/council/planning/applicationTypeCode>
      rdf:type rdf:Property ;
      rdfs:label "Application type code"^^xsd:string ;
	  rdfs:comment "Short form version of the application type." ;
      rdfs:domain <http://data.gmdsp.org.uk/def/council/planning/PlanningApplication> ;
      rdfs:range xsd:string .

<http://data.gmdsp.org.uk/def/council/planning/developmentType>
      rdf:type rdf:Property ;
      rdfs:label "Development type"^^xsd:string ;
	  rdfs:comment "Development type of the application eg advertisement." ;
      rdfs:domain <http://data.gmdsp.org.uk/def/council/planning/PlanningApplication> ;
      rdfs:range xsd:string .

<http://data.gmdsp.org.uk/def/council/planning/proposal>
      rdf:type rdf:Property ;
      rdfs:label "Proposal"^^xsd:string ;
	  rdfs:comment "Free text description of the proposal in the planning application." ;
      rdfs:domain <http://data.gmdsp.org.uk/def/council/planning/PlanningApplication> ;
      rdfs:range xsd:string .

<http://data.gmdsp.org.uk/def/council/planning/hasDistrictWard>
      rdf:type rdf:Property ;
      rdfs:label "Proposal"^^xsd:string ;
	  rdfs:comment "Free text description of the proposal in the planning application." ;
      rdfs:domain <http://data.gmdsp.org.uk/def/council/planning/PlanningApplication> ;
      rdfs:range <http://data.ordnancesurvey.co.uk/ontology/admingeo/DistrictWard> .